commit

Workbench.v
@@ -4,6 +4,9 @@ Import SnoclistNotations.
 Require Import PlanarLambda.
 Require Import Types.
 
+Require Import Coq.Program.Equality.
+Require Import Arith.
+Require Import Coq.Logic.JMeq.
 Require List.
 
 Definition context n : Type := snoclist type n.
@@ -21,46 +24,239 @@ Inductive is_typed : forall {a : nat}, context a -> pterm a -> type -> Prop :=
 Definition s_rule : Type := nat * type.
 Definition s_rules : Type := list s_rule.
 
-Fixpoint subst (rul : s_rule) (ty : type) : type :=
+Fixpoint subst1_ty (rul : s_rule) (ty : type) : type :=
 match ty with
 | TVar n => let (m, u) := rul in
   match eqb n m with
   | true => u
   | false => ty
   end
-| TImp ty1 ty2 => TImp (subst rul ty1) (subst rul ty2)
+| TImp ty1 ty2 => TImp (subst1_ty rul ty1) (subst1_ty rul ty2)
 end.
 
 Fixpoint subst_ty (sigma : s_rules) (ty : type) : type :=
 match sigma with
 | List.nil => ty
 | List.cons rul sigma' =>
-  subst_ty sigma' (subst rul ty)
+  subst_ty sigma' (subst1_ty rul ty)
+end.
+
+Fixpoint subst1_ctx {n : nat} (rul : s_rule) (ctx : context n) : context n :=
+match ctx with
+| [] => []
+| ctx' :: ty => (subst1_ctx rul ctx') :: (subst1_ty rul ty)
 end.
 
 Fixpoint subst_ctx {n : nat} (sigma : s_rules) (ctx : context n) : context n :=
-match ctx with
-| [] => []
-| ctx' :: ty => (subst_ctx sigma ctx') :: (subst_ty sigma ty)
+match sigma with
+| List.nil => ctx
+| List.cons rul sigma' =>
+  subst_ctx sigma' (subst1_ctx rul ctx)
 end.
+
+
+Inductive pterm_eq : forall {a : nat}, pterm a -> pterm a -> Prop :=
+| eq_var : pterm_eq PVar PVar
+| eq_abs {n} (tl tr : pterm (S n)) :
+  pterm_eq tl tr -> pterm_eq (PAbs tl) (PAbs tr)
+| eq_app {n m} (tl1 : pterm n) (tl2 : pterm m) (tr1 : pterm n) (tr2 : pterm m) :
+  pterm_eq tl1 tr1 -> pterm_eq tl2 tr2 -> pterm_eq (PApp tl1 tl2) (PApp tr1 tr2)
+| eq_sym {n} (tl tr : pterm n) : pterm_eq tl tr -> pterm_eq tr tl
+| eq_trans {n} (tl tm tr : pterm n) :
+  pterm_eq tl tm -> pterm_eq tm tr -> pterm_eq tl tr.
+
+Lemma pt_eq : forall {a : nat} (t1 t2 : pterm a), t1 = t2 <-> pterm_eq t1 t2.
+Proof.
+intros a t1 t2. split.
+- intro eq. 
+  induction t2.
+  + rewrite eq. apply eq_var.
+  + rewrite eq.
+    apply (eq_abs t2 t2 (IHt2 t2 eq_refl)).
+  + rewrite eq.
+    apply (eq_app t2_1 t2_2 t2_1 t2_2 (IHt2_1 t2_1 eq_refl) (IHt2_2 t2_2 eq_refl)).
+- intro pt_eq.
+  induction pt_eq.
+  + apply eq_refl.
+  + rewrite IHpt_eq. apply eq_refl.
+  + rewrite IHpt_eq1. rewrite IHpt_eq2. apply eq_refl.
+  + rewrite IHpt_eq. apply eq_refl.
+  + rewrite IHpt_eq1. rewrite IHpt_eq2. apply eq_refl.
+Qed.
+
+Inductive pterm_JMeq : forall {a b : nat}, pterm a -> pterm b -> Prop :=
+| JMeq_var : pterm_JMeq PVar PVar
+| JMeq_abs {n m} (tl : pterm (S n)) (tr : pterm (S m)) :
+  pterm_JMeq tl tr -> pterm_JMeq (PAbs tl) (PAbs tr)
+| JMeq_app {nl nr ml mr} (tl1 : pterm nl) (tl2 : pterm ml) (tr1 : pterm nr) (tr2 : pterm mr) :
+  pterm_JMeq tl1 tr1 -> pterm_JMeq tl2 tr2 -> pterm_JMeq (PApp tl1 tl2) (PApp tr1 tr2)
+| JMeq_sym {n m} (tl : pterm n) (tr : pterm m) : pterm_JMeq tl tr -> pterm_JMeq tr tl
+| JMeq_trans {n m p} (tl : pterm n) (tm : pterm m) (tr : pterm p) :
+  pterm_JMeq tl tm -> pterm_JMeq tm tr -> pterm_JMeq tl tr
+| JMeq_refl {n} (t : pterm n) : pterm_JMeq t t.
+
+Lemma pterm_JMeq_is_eq : forall {a b : nat} (t1 : pterm a) (t2 : pterm b),
+  pterm_JMeq t1 t2 -> a = b.
+Proof. intros a b t1 t2 h.
+induction h.
+- reflexivity.
+- apply (eq_add_S n m IHh).
+- apply (f_equal2_plus nl nr ml mr IHh1 IHh2).
+- apply (Nat.eq_sym IHh).
+- apply (Nat.eq_trans IHh1 IHh2).
+- reflexivity.
+Qed.
+
+Import EqNotations.
+
+Lemma pterm_JMeq_refl : forall {a : nat} (t : pterm a), pterm_JMeq t t.
+Admitted.
+
+Check eq_ind.
+
+Lemma pt_ind : forall {n : nat} {x : pterm n} (P : forall {n' : nat}, pterm n' -> Prop),
+  P x -> forall {m : nat} {y : pterm m}, n = m -> JMeq x y -> P y.
+Admitted.
+
+Lemma pt_JMeq : forall {a b : nat} (t1 : pterm a) (t2 : pterm b), JMeq t1 t2 <-> pterm_JMeq t1 t2.
+Admitted.
+
+
+Lemma subst1_typed : forall {n : nat} (rul : s_rule) (ctx : context n) (pt : pterm n) (ty : type),
+  is_typed ctx pt ty -> is_typed (subst1_ctx rul ctx) pt (subst1_ty rul ty).
+Proof.
+intro n.
+case_eq n.
+- intro eq. intros rul ctx pt ty.
+  dependent destruction ctx.
+  case ty.
+  case rul.
+  + intros target ty' atom h.
+    dependent destruction pt.
+    dependent destruction h.
+Admitted.
 
 Lemma subst_typed : forall {n : nat} (sigma : s_rules) (ctx : context n) (pt : pterm n) (ty : type),
   is_typed ctx pt ty -> is_typed (subst_ctx sigma ctx) pt (subst_ty sigma ty).
-Admitted.
+Proof.
+intros n sigma.
+induction sigma.
+- simpl. intros ctx pt ty h. apply h.
+- simpl. intros ctx pt ty h. apply IHsigma. apply subst1_typed. apply h.
+Qed.
 
 Definition is_princ : Type := forall {n : nat} (ctx : context n) (pt : pterm n) (ty : type),
   is_typed ctx pt ty -> forall (ctx' : context n) (ty' : type), is_typed ctx' pt ty' ->
   sig (fun (sigma : s_rules) => ctx' = subst_ctx sigma ctx /\ ty' = subst_ty sigma ty).
 
-(* ===== Inference ===== *)
+(* ===== Labeled Terms ===== *)
+
+Inductive sterm : nat -> Type :=
+| SAbs {n} : sterm (S n) -> sterm n
+| SCir {n} : nat -> cterm n -> sterm n
+
+with cterm : nat -> Type :=
+| CVar : cterm 1
+| CApp {n} {m} : cterm n -> sterm m -> cterm (n + m)
+| CSqu {n} : sterm n -> cterm n.
+
+Inductive lterm : nat -> Type :=
+| LSyn {n} : sterm n -> lterm n
+| LChk {n} : cterm n -> lterm n.
+
+Fixpoint strip_syn {n : nat} (t : sterm n) : pterm n :=
+match t with
+| SAbs t' => PAbs (strip_syn t')
+| SCir a t' => strip_chk t'
+end
+with strip_chk {n : nat} (t : cterm n) : pterm n :=
+match t with
+| CVar => PVar
+| CApp ct st => PApp (strip_chk ct) (strip_syn st)
+| CSqu t' => strip_syn t'
+end.
+
+Definition strip_labels {n : nat} (t : lterm n) : pterm n :=
+match t with
+| LSyn st => strip_syn st
+| LChk ct => strip_chk ct
+end.
+
+(*
+Inductive is_typed : forall {a : nat}, context a -> pterm a -> type -> Prop :=
+| typed_var ty : is_typed [ty] PVar ty
+| typed_abs {n} ty1 gamma (pt : pterm (S n)) ty2 :
+  is_typed (gamma :: ty1) pt ty2 -> is_typed gamma (PAbs pt) (TImp ty1 ty2)
+| typed_app {n m} gamma delta (pt1 : pterm n) (pt2 : pterm m) ty1 ty2:
+  is_typed gamma pt1 (TImp ty1 ty2) -> is_typed delta pt2 ty1 ->
+  is_typed (gamma ++ delta) (PApp pt1 pt2) ty2.
+*)
 
 Definition type_eq : Type := type * type.
 Definition constraints : Type := list type_eq.
 
-Definition length {A : Type} {n : nat} : snoclist A n -> nat := fix length l := n.
+Inductive is_bidir_syn : forall {a : nat}, context a -> sterm a -> type -> constraints -> Prop :=
+| bidir_abs {n} ty1 gamma (st : sterm (S n)) ty2 const :
+  is_bidir_syn (gamma :: ty1) st ty2 const -> 
+  is_bidir_syn  gamma (SAbs st) (TImp ty1 ty2) const
+| bidir_cir {n} (a : nat) gamma (ct : cterm n) ty const :
+  is_bidir_chk gamma ct ty const ->
+  is_bidir_syn gamma (SCir a ct) ty const
 
-(*Check let (pair a b, c) := (pair 1 2, 3) in a.*)
+with is_bidir_chk : forall {a : nat}, context a -> cterm a -> type -> constraints -> Prop :=
+| bidir_var ty : is_bidir_chk [ty] CVar ty List.nil
+| bidir_app {n m} gamma delta (ct1 : cterm n) (st2 : sterm m) ty1 ty2 const1 const2 :
+  is_bidir_chk gamma ct1 (TImp ty1 ty2) const1 ->
+  is_bidir_syn delta st2 ty1 const2 ->
+  is_bidir_chk (gamma ++ delta) (CApp ct1 st2) ty2 (List.app const1 const2)
+| bidir_squ {n} gamma (st : sterm n) ty1 ty2 const :
+  is_bidir_syn gamma st ty1 const ->
+  is_bidir_chk gamma (CSqu st) ty2 (List.cons (ty1, ty2) const).
 
+Inductive is_bidir : forall {a : nat}, context a -> lterm a -> type -> constraints -> Prop :=
+| Sbidir {n} gamma (st : sterm n) ty const :
+  is_bidir_syn gamma st ty const ->
+  is_bidir gamma (LSyn st) ty const
+| Cbidir {n} gamma (ct : cterm n) ty const :
+  is_bidir_chk gamma ct ty const ->
+  is_bidir gamma (LChk ct) ty const.
+
+(*
+Lemma typed_lp : forall {a : nat} (ctx : context a) (lt : lterm a) (ty : type) (const : constraints),
+  is_bidir ctx lt ty const -> is_typed ctx (strip_labels lt) ty.
+Proof.
+intros a ctx lt ty const.
+induction lt.
+induction s.
+intro h.
+case ty in h.
+induction h.
+- 
+  case_eq ty.
+  + admit.
+  + simpl. apply 
+*)
+
+(* ===== Inference ===== *)
+
+
+
+
+
+
+(*
+Inductive b_synth : forall {a : nat} (newout : nat), context a -> pterm a -> type -> constraints -> Prop :=
+| syn_var (ctx : context 1) :
+  chk_test newout ctx PVar (S newout)
+| syn_test ty : b_synth  0 [ty] PVar ty List.nil
+
+with b_check : forall {a : nat} (newin : nat), context a -> pterm a -> type -> constraints -> Prop :=
+| chk_test ty : b_check 0 [ty] PVar ty List.nil.
+*)
+
+
+
+(*
 Fixpoint Bidir_synth {n : nat} (fresh : nat) (t : pterm n) : (nat * context n * type * constraints) :=
 match t in pterm n return (nat * context n * type * constraints) with
 | PAbs t' =>
@@ -97,6 +293,8 @@ match t in pterm n return (nat * context n * constraints) with
   let (fresh', ctx') := temp' in
   (fresh', ctx', List.cons (A, ty) const)
 end.
+
+*)
 
 
 
