README.txt
@@ -9,10 +9,14 @@ make -f CoqMakeFile clean
 
 - substitution
 - type substitution
-- proof of subst_typed
-- change bidir into a predicate
+- proof of subst_typed (Subproofs Left)
+
+
+- change bidir into a predicate (Postponed and the below are priority)
 - add shape-annotated planar lambda-terms
 - do shape annotated bidir
+
+
 - some predicate on the principal typing
 - sigma satisfies constraints
 
